new-semantics/coq/events/LinkDefs.v
@@ -58,6 +58,20 @@ Section LinkDefs.
     (nInσ0 : ~ In ℓ (floc_nv σ0))
     (LINKv : link σ0 (open_loc_vl 0 (ℓ, p) v) v')
   : link σ0 (wvl_recv p v) (wvl_recv p (close_vl 0 (ℓ, p) v'))
+  | link_nat n
+  : link σ0 (vl_nat n) (vl_nat n)
+  | link_succNat (E : vnt _ _ _ _) n
+    (LINKE : link σ0 E (vl_nat n))
+  : link σ0 (SuccE E) (vl_nat (S n))
+  | link_succEvent (E E' : vnt _ _ _ _)
+    (LINKE : link σ0 E E')
+  : link σ0 (SuccE E) (SuccE E')
+  | link_predNat (E : vnt _ _ _ _) n
+    (LINKE : link σ0 E (vl_nat (S n)))
+  : link σ0 (PredE E) (vl_nat n)
+  | link_predEvent (E E' : vnt _ _ _ _)
+    (LINKE : link σ0 E E')
+  : link σ0 (PredE E) (PredE E')
   .
 End LinkDefs.
 
