new-semantics/coq/playground/ShadowInterpreter.v
@@ -1,0 +1,175 @@
+From Coq Require Import ZArith String List.
+Import ListNotations.
+
+Local Open Scope string_scope.
+
+Inductive tm :=
+  | Var (x : string)
+  | Fn (x : string) (e : tm)
+  | App (f a : tm)
+  | Link (m e : tm)
+  | Mt
+  | Bind (x : string) (v m : tm)
+.
+
+Inductive env :=
+  | No_shadow (β : list (string * val))
+    (* no shadow at the bottom *)
+  | Shadow_env (β : list (string * val)) (s : shadow)
+    (* shadow at the bottom *)
+
+with val :=
+  | Clos (x : string) (k : option val) (σ : env)
+  | Mod (σ : env)
+  | Shadow_val (s : shadow)
+
+with shadow :=
+  | Init
+  | Read (s : shadow) (x : string)
+  | Call (s : shadow) (v : val)
+.
+
+Local Coercion Var : string >-> tm.
+Local Notation "'⟪' 'λ' x e '⟫'" := (Fn x e) (at level 60, right associativity).
+Local Notation "'⟪' '@' M N '⟫'" := (App M N) (at level 60, right associativity).
+Local Notation "'⟪' M '⋊' N '⟫'" := (Link M N) (at level 60, right associativity).
+Local Notation "'⟪' ε '⟫'" := (Mt) (at level 60, right associativity).
+Local Notation "'⟪' x '=' M ';' N '⟫'" := (Bind x M N) (at level 60, right associativity).
+
+Definition ω := Fn "x" (App (Var "x") (Var "x")).
+Definition ι := Fn "x" (Var "x").
+
+Definition upd_env (σ : env) (x : string) (v : val) :=
+  match σ with
+  | No_shadow β => No_shadow ((x, v) :: β)
+  | Shadow_env β s => Shadow_env ((x, v) :: β) s
+  end.
+
+Definition app_env β σ :=
+  match σ with
+  | No_shadow β' => No_shadow (β ++ β')
+  | Shadow_env β' s => Shadow_env (β ++ β') s
+  end.
+
+Fixpoint read_list (β : list (string * val)) (x : string) :=
+  match β with
+  | [] => None
+  | (x', v) :: β' =>
+    if x =? x' then Some v else read_list β' x
+  end.
+
+Definition read_env (σ : env) (x : string) :=
+  match σ with
+  | No_shadow β => read_list β x
+  | Shadow_env β s =>
+    match read_list β x with
+    | Some v => Some v
+    | None => Some (Shadow_val (Read s x))
+    end
+  end.
+
+Definition eval (link : env -> val -> option val) :=
+  fix eval (e : tm) : option val :=
+  match e with
+  | Var x => Some (Shadow_val (Read Init x))
+  | Fn x M => Some (Clos x (eval M) (Shadow_env [] Init))
+  | App M N =>
+    match eval M, eval N with
+    | Some (Clos x B σ), Some v =>
+      match B with
+      | Some k => link (upd_env σ x v) k
+      | None => None
+      end
+    | Some (Shadow_val s), Some v => Some (Shadow_val (Call s v))
+    | Some (Mod _), Some _
+    | Some _, None | None, Some _ | None, None => None
+    end
+  | Link M N =>
+    match eval M, eval N with
+    | Some (Mod σ), Some v => link σ v
+    | Some (Shadow_val s), Some v => link (Shadow_env [] s) v
+    | Some (Clos _ _ _), Some _
+    | Some _, None | None, Some _ | None, None => None
+    end
+  | Mt => Some (Mod (No_shadow []))
+  | Bind x M N =>
+    match eval M, eval N with
+    | Some v, Some (Mod σ) => Some (Mod (upd_env σ x v))
+    | Some v, Some (Shadow_val s) => Some (Mod (Shadow_env [(x, v)] s))
+    | Some _, Some (Clos _ _ _)
+    | Some _, None | None, Some _ | None, None => None
+    end
+  end.
+
+(* linking, up to n steps *)
+Fixpoint link (n : nat) (σ : env) : val -> option val :=
+  match n with 0 => (fun _ => None) | S n =>
+  fix link_val v : option val :=
+    match v with
+    | Clos x k σ' =>
+      match link_env σ' with
+      | None => None
+      | Some σ' => Some (Clos x k σ')
+      end
+    | Mod σ' =>
+      match link_env σ' with
+      | None => None
+      | Some σ' => Some (Mod σ')
+      end
+    | Shadow_val s => link_shadow s
+    end
+  with link_env σ' : option env :=
+    let fix link_list β :=
+      match β with
+      | [] => Some []
+      | (x, v) :: β =>
+        match link_val v, link_list β with
+        | None, _ | _, None => None
+        | Some v, Some β => Some ((x, v) :: β)
+        end
+      end
+    in match σ' with
+    | No_shadow β =>
+      match link_list β with None => None | Some β => Some (No_shadow β) end
+    | Shadow_env β s =>
+      match link_list β, link_shadow s with
+      | None, _ | _, None => None
+      | Some _, Some (Clos _ _ _) => None
+      | Some β, Some (Mod σ) => Some (app_env β σ)
+      | Some β, Some (Shadow_val s) => Some (Shadow_env β s)
+      end
+    end
+  with link_shadow s : option val :=
+    match s with
+    | Init => Some (Mod σ)
+    | Read s x =>
+      match link_shadow s with
+      | None | Some (Clos _ _ _) => None
+      | Some (Mod σ) => read_env σ x
+      | Some (Shadow_val s) => Some (Shadow_val (Read s x))
+      end
+    | Call s v =>
+      match link_shadow s, link_val v with
+      | None, _ | _, None | Some (Mod _), _ => None
+      | Some (Clos x k σ), Some v =>
+        match k with
+        | None => None
+        | Some k => link n (upd_env σ x v) k
+        end
+      | Some (Shadow_val s), Some v => Some (Shadow_val (Call s v))
+      end
+    end
+  for link_val
+  end.
+
+Definition interp n := eval (link n).
+
+Local Coercion Shadow_val : shadow >-> val.
+Local Coercion Mod : env >-> val.
+Compute interp 1 ω.
+Compute interp 100 (App ω ω).
+Compute interp 1 (App ι ι).
+Definition test_module := Bind "id" ι Mt.
+Definition open_program := App (Var "id") (Var "id").
+Compute interp 2 (Link test_module open_program).
+
